src/SDK/Keyring/MultiKeyring.dfy
@@ -27,14 +27,18 @@ module {:extern "MultiKeyringDef"} MultiKeyringDef {
         constructor (g : Keyring?, c : seq<Keyring>) ensures generator == g ensures children == c
             requires g != null ==> g.Valid()
             requires forall i :: 0 <= i < |c| ==> c[i].Valid()
-            ensures Valid()
+            ensures Valid() && fresh(Repr - (if g != null then g.Repr else {}) - childrenRepr(c))
         {
             generator := g;
             children := c;
-            Repr := {this} + (if g != null then {g} + g.Repr else {}) + childrenRepr(c);
+            Repr := {this} + (if g != null then g.Repr else {}) + childrenRepr(c);
         }
 
-        predicate Valid() reads this, Repr {
+        predicate Valid()
+          reads this, Repr
+          ensures Valid() ==> this in Repr
+        {
+            && this in Repr
             && (generator != null ==> generator in Repr && generator.Repr <= Repr && generator.Valid())
             && (forall j :: 0 <= j < |children| ==> children[j] in Repr && children[j].Repr <= Repr && children[j].Valid())
         }
