src/SDK/CMM/Defs.dfy
@@ -13,8 +13,10 @@ module {:extern "CMMDefs"} CMMDefs {
   import MessageHeader
 
   trait {:termination false} CMM {
-    ghost var Repr : set<object>
-    predicate Valid() reads this, Repr
+    ghost var Repr: set<object>
+    predicate Valid()
+      reads this, Repr
+      ensures Valid() ==> this in Repr
 
     method GetEncryptionMaterials(materialsRequest: Materials.EncryptionMaterialsRequest)
                                   returns (res: Result<Materials.ValidEncryptionMaterials>)
